providers/test/Test.Hash.fst
@@ -9,9 +9,7 @@ module MP = LowStar.ModifiesPat
 
 open LowStar.BufferOps
 
-open ST
-
-let main (): St unit =
+let main (): ST.St unit =
   let s1 = H.create H.SHA256 in
   let h1 = ST.get () in
   let s2 = H.create H.SHA384 in
